providers/evercrypt/EverCrypt.CTR.fsti
@@ -56,6 +56,7 @@ val frame_invariant: #a:alg -> l:B.loc -> s:state a -> h0:HS.mem -> h1:HS.mem ->
   (ensures (
     invariant h1 s /\
     footprint h0 s == footprint h1 s))
+  [ SMTPat (invariant h1 s); SMTPat (B.modifies l h0 h1) ]
 
 /// Ghost accessors
 /// ---------------
@@ -97,8 +98,10 @@ let create_in_st (a:alg) =
       B.live h0 dst /\ B.live h0 k /\ B.live h0 nonce)
     (ensures fun h0 e h1 ->
       match e with
-      | UnsupportedAlgorithm | InvalidIVLength ->
+      | UnsupportedAlgorithm ->
           B.(modifies loc_none h0 h1)
+      | InvalidIVLength ->
+          B.(modifies loc_none h0 h1) /\ UInt32.v nonce_len < 12
       | Success ->
           let s = B.deref h1 dst in
           // Sanity
